verif/verif_movetofirst.v
@@ -1,0 +1,48 @@
+(** * verif_movetofirst.v : Correctness proof of moveToFirst *)
+
+Require Import VST.floyd.proofauto.
+Require Import VST.floyd.library.
+Require Import relation_mem.
+Instance CompSpecs : compspecs. make_compspecs prog. Defined.
+Definition Vprog : varspecs. mk_varspecs prog. Defined.
+
+Require Import VST.msl.wand_frame.
+Require Import VST.msl.iter_sepcon.
+Require Import VST.floyd.reassoc_seq.
+Require Import VST.floyd.field_at_wand.
+Require Import FunInd.
+Require Import btrees.
+Require Import btrees_sep.
+Require Import btrees_spec.
+Require Import index.
+
+Lemma body_moveToFirst: semax_body Vprog Gprog f_moveToFirst moveToFirst_spec.
+Proof.
+  start_function.
+  forward_if (
+      PROP(pn<>nullval)
+      LOCAL(temp _cursor pc; temp _node pn; temp _level (Vint (Int.repr (Zlength c))))
+      SEP(relation_rep r pr; cursor_rep c r pc))%assert.
+  - admit.
+  - forward.                    (* skip *)
+    entailer!.
+  - assert_PROP(False).
+    entailer!.                  (* contradiction in H2? *)
+    admit.
+    inv H3.
+  - forward_if (
+        (PROP (pn <> nullval; pc <> nullval)
+         LOCAL (temp _cursor pc; temp _node pn; temp _level (Vint (Int.repr (Zlength c))))
+         SEP (relation_rep r pr; cursor_rep c r pc))).
+    + forward. entailer!.
+    + assert_PROP(False).
+      entailer. inv H4.
+    + forward_if ((PROP (pn <> nullval; pc <> nullval; (Zlength c) >= 0)
+     LOCAL (temp _cursor pc; temp _node pn; temp _level (Vint (Int.repr (Zlength c))))
+     SEP (relation_rep r pr; cursor_rep c r pc))).
+      * forward. entailer!.
+      * assert_PROP(False). entailer.
+        (* contradiction in H2. *) admit.
+        inv H5.
+      * admit.
+Admitted.
